src/InvariantProofs.v
@@ -21,42 +21,6 @@
 Require Import Rcore RfeaturesAux Rinit.
 Require Export Invariants.
 
-(** * General Lemmae **)
-
-(** If runs returns a result, then adding fuel does not change it. **)
-Lemma runs_while_loop_fuel_conserve : forall A globals n n' S (a : A) expr body,
-    n <= n' ->
-    ~ bottom_result (runs_while_loop (runs n globals) S a expr body) ->
-    runs_while_loop (runs n' globals) S a expr body = runs_while_loop (runs n globals) S a expr body.
-Proof.
-  introv I B. repeat rewrite <- runs_proj_while_loop_eq in *. gen n' S a. induction n; introv I B.
-  - false~ B.
-  - destruct n'; try solve [ math ]. simpls. unfolds while_loop. repeat rewrite <- runs_proj_while_loop_eq.
-    destruct expr; simpls~; tryfalse~. cases_if~.
-    destruct body; simpls~; tryfalse~. rewrite~ IHn. math.
-Qed.
-
-(* Slow version
-Lemma runs_while_loop_fuel_conserve : forall A globals n n' S (a : A) expr body,
-    n <= n' ->
-    ~ bottom_result (runs_while_loop (runs n globals) S a expr body) ->
-    runs_while_loop (runs n' globals) S a expr body = runs_while_loop (runs n globals) S a expr body.
-Proof.
-  introv I B. gen n' S a. induction n; introv I B.
-  - false~ B.
-  - destruct n'; try solve [ math ]. simpls. unfolds while_loop. repeat rewrite <- runs_proj_while_loop_eq.
-    destruct expr; simpls~; tryfalse~. cases_if~.
-    destruct body; simpls~; tryfalse~. rewrite~ IHn. math.
-Qed.
-*)
-
-(* TODO: put these lemmae in RfeaturesAux.v.
-   In RfeaturesAux, we can change the tactic to work on all projections
-   by only unfolding everything in aux1 (no simplifications), then do a
-   simplification between the two auxn.
-   We will then be able to automate the lemmae above, without them taking
-   too much time to compile. *)
-
 (** * Lemmae about Rinit.v **)
 
 (* TODO *)
